src/dvspec/dafny/att_spec_proofs/dvn_init_inv.dfy
@@ -38,7 +38,7 @@ module DVN_Init_Inv
         }        
     }
 
-    lemma lemma_invs_1_to_10_dvn_init(dvn: DVState)       
+    lemma lemma_invs_1_to_15_dvn_init(dvn: DVState)       
     requires DV.Init(dvn, {})    
     ensures inv1(dvn)
     ensures inv2(dvn)
@@ -51,6 +51,10 @@ module DVN_Init_Inv
     ensures inv9(dvn)
     ensures inv10(dvn)
     ensures inv11(dvn)
+    ensures inv12(dvn)
+    ensures inv13(dvn)
+    ensures inv14(dvn)    
+    ensures inv15(dvn)    
     {}  
     
 
