src/dvspec/dafny/att_spec_proofs/dvn_next_inv.dfy
@@ -21,39 +21,19 @@ module DVN_Next_Inv
     import opened Fnc_Inv
     import opened Helper_Sets_Lemmas
 
-    
-
-    lemma lemma_inv1_dvn_next(dvn: DVState, dvn': DVState)       
-    requires exists e: DV.Event :: DV.NextEvent(dvn, e, dvn')
-    requires inv1(dvn)
-    ensures inv1(dvn')
-    { }
-
-    lemma lemma_inv1_dvn_next2(dvn: DVState, event: DV.Event, dvn': DVState)       
+    lemma lemma_inv1_dvn_next(dvn: DVState, event: DV.Event, dvn': DVState)       
     requires DV.NextEvent(dvn, event, dvn')
     requires inv1(dvn)
     ensures inv1(dvn')
     { }    
 
-    lemma lemma_inv2_dvn_next(dvn: DVState, dvn': DVState)       
-    requires exists e: DV.Event :: DV.NextEvent(dvn, e, dvn')
-    requires inv2(dvn)
-    ensures inv2(dvn')
-    { }
-
-    lemma lemma_inv2_dvn_next2(dvn: DVState, event: DV.Event, dvn': DVState)       
+    lemma lemma_inv2_dvn_next(dvn: DVState, event: DV.Event, dvn': DVState)       
     requires DV.NextEvent(dvn, event, dvn')
     requires inv2(dvn)
     ensures inv2(dvn')
     { }    
 
-    lemma lemma_inv3_dvn_next(dvn: DVState, dvn': DVState)       
-    requires exists e: DV.Event :: DV.NextEvent(dvn, e, dvn')
-    requires inv3(dvn)
-    ensures inv3(dvn')
-    { }
-
-    lemma lemma_inv3_dvn_next2(dvn: DVState, event: DV.Event, dvn': DVState)       
+    lemma lemma_inv3_dvn_next(dvn: DVState, event: DV.Event, dvn': DVState)       
     requires DV.NextEvent(dvn, event, dvn')
     requires inv3(dvn)
     ensures inv3(dvn')
@@ -422,40 +402,147 @@ module DVN_Next_Inv
         }   
     }  
 
-    // It takes more than 60 seconds to prove lemma_inv11_dvn_next.
+    
     lemma lemma_inv11_dvn_next(
         dvn: DVState,
         event: DV.Event,
         dvn': DVState
     )    
     requires NextEvent(dvn, event, dvn')    
-    requires inv8(dvn)
     requires inv11(dvn)
-    ensures inv11(dvn')
+    ensures inv11(dvn)
+    { }
+
+    lemma lemma_inv12_dvn_next(
+        dvn: DVState,
+        event: DV.Event,
+        dvn': DVState
+    )    
+    requires NextEvent(dvn, event, dvn')  
+    requires inv1(dvn)  
+    requires inv4(dvn)
+    requires inv11(dvn)
+    requires inv12(dvn)
+    ensures inv12(dvn')
+    {   
+        var queue := dvn'.sequence_attestation_duties_to_be_served;
+        var index := dvn'.index_next_attestation_duty_to_be_served;        
+        var next_duty := queue[index].attestation_duty;
+        var hn := queue[index].node;
+
+        if hn in dvn'.honest_nodes_states.Keys 
+        {
+            var dvc' := dvn'.honest_nodes_states[hn];
+
+            lemma_inv4_dvn_next(dvn, event, dvn');
+            assert inv4(dvn');
+
+            lemma_inv11_dvn_next(dvn, event, dvn');
+            assert inv11(dvn');
+
+            forall rcvd_duty: AttestationDuty | rcvd_duty in dvc'.all_rcvd_duties
+            ensures rcvd_duty.slot <= next_duty.slot
+            {
+                var k: nat :| && 0 <= k < dvn'.index_next_attestation_duty_to_be_served
+                              && dvn'.sequence_attestation_duties_to_be_served[k].node == hn
+                              && dvn'.sequence_attestation_duties_to_be_served[k].attestation_duty == rcvd_duty;
+
+                assert dvn'.sequence_attestation_duties_to_be_served[k].attestation_duty.slot <= next_duty.slot;
+
+                assert rcvd_duty.slot <= next_duty.slot;
+            }
+
+            assert inv12_body(dvc', next_duty);
+        }
+    } 
+
+    lemma lemma_inv13_dvn_next(
+        dvn: DVState,
+        event: DV.Event,
+        dvn': DVState
+    )    
+    requires NextEvent(dvn, event, dvn')  
+    requires inv1(dvn)  
+    requires inv4(dvn)
+    requires inv5(dvn)
+    requires inv11(dvn)
+    requires inv12(dvn)
+    requires inv13(dvn)
+    ensures inv13(dvn')
+    {   
+        var queue := dvn'.sequence_attestation_duties_to_be_served;
+        var index := dvn'.index_next_attestation_duty_to_be_served;        
+        var next_duty := queue[index].attestation_duty;
+        var hn := queue[index].node;
+
+        if hn in dvn'.honest_nodes_states.Keys 
+        {
+            var dvc' := dvn'.honest_nodes_states[hn];
+
+            lemma_inv4_dvn_next(dvn, event, dvn');
+            assert inv4(dvn');
+
+            lemma_inv5_dvn_next(dvn, event, dvn');
+            assert inv5(dvn');
+
+            lemma_inv11_dvn_next(dvn, event, dvn');
+            assert inv11(dvn');
+
+            lemma_inv12_dvn_next(dvn, event, dvn');
+            assert inv12(dvn');
+
+            forall rcvd_duty: AttestationDuty | rcvd_duty in dvc'.attestation_duties_queue
+            ensures rcvd_duty.slot <= next_duty.slot
+            {
+                assert rcvd_duty in dvc'.all_rcvd_duties;
+
+                var k: nat :| && 0 <= k < dvn'.index_next_attestation_duty_to_be_served
+                              && dvn'.sequence_attestation_duties_to_be_served[k].node == hn
+                              && dvn'.sequence_attestation_duties_to_be_served[k].attestation_duty == rcvd_duty;
+
+                assert dvn'.sequence_attestation_duties_to_be_served[k].attestation_duty.slot <= next_duty.slot;
+
+                assert rcvd_duty.slot <= next_duty.slot;
+            }
+
+            assert inv13_body(dvc', next_duty);
+        }
+    }
+
+    // It takes more than 60 seconds to prove lemma_inv14_dvn_next.
+    lemma lemma_inv14_dvn_next(
+        dvn: DVState,
+        event: DV.Event,
+        dvn': DVState
+    )    
+    requires NextEvent(dvn, event, dvn')    
+    requires inv8(dvn)
+    requires inv14(dvn)
+    ensures inv14(dvn')
     {        
         match event 
         {
             case HonestNodeTakingStep(node, nodeEvent, nodeOutputs) =>
                 var dvc := dvn.honest_nodes_states[node];
                 var dvc' := dvn'.honest_nodes_states[node];
-                assert inv11_body(dvc);
+                assert inv14_body(dvc);
                 match nodeEvent
                 {
                     case ServeAttstationDuty(attestation_duty) =>                             
-                        lemma_inv11_f_serve_attestation_duty(dvc, attestation_duty, dvc');
+                        lemma_inv14_f_serve_attestation_duty(dvc, attestation_duty, dvc');
                         
                     case AttConsensusDecided(id, decided_attestation_data) => 
-                        lemma_inv11_f_att_consensus_decided(dvc, id, decided_attestation_data, dvc');                                                
+                        lemma_inv14_f_att_consensus_decided(dvc, id, decided_attestation_data, dvc');                                                
                         
                     case ReceviedAttesttionShare(attestation_share) =>                         
-                        lemma_inv11_f_listen_for_attestation_shares(dvc, attestation_share, dvc');                        
+                        lemma_inv14_f_listen_for_attestation_shares(dvc, attestation_share, dvc');                        
    
                     case ImportedNewBlock(block) => 
                         var dvc_mod := add_block_to_bn(dvc, nodeEvent.block);
-                        lemma_inv11_add_block_to_bn(dvc, nodeEvent.block, dvc_mod);
-                        assert inv11_body(dvc_mod);
-                        lemma_inv11_f_listen_for_new_imported_blocks(dvc_mod, block, dvc');                        
-                        assert inv11_body(dvc');
+                        lemma_inv14_add_block_to_bn(dvc, nodeEvent.block, dvc_mod);
+                        assert inv14_body(dvc_mod);
+                        lemma_inv14_f_listen_for_new_imported_blocks(dvc_mod, block, dvc');                        
+                        assert inv14_body(dvc');
                         
                     case ResendAttestationShares =>                                                                      
 
@@ -468,6 +555,55 @@ module DVN_Next_Inv
         }   
     }  
 
-    
+    lemma lemma_inv15_dvn_next(
+        dvn: DVState,
+        event: DV.Event,
+        dvn': DVState
+    )    
+    requires NextEvent(dvn, event, dvn')  
+    requires inv1(dvn)  
+    requires inv2(dvn)
+    requires inv4(dvn)
+    requires inv5(dvn)
+    requires inv11(dvn)
+    requires inv13(dvn)
+    requires inv15(dvn)
+    ensures inv15(dvn')
+    {        
+        match event 
+        {
+            case HonestNodeTakingStep(node, nodeEvent, nodeOutputs) =>
+                var dvc := dvn.honest_nodes_states[node];
+                var dvc' := dvn'.honest_nodes_states[node];
+                
+                
+                match nodeEvent
+                {
+                    case ServeAttstationDuty(attestation_duty) =>                                                                     
+                        lemma_inv15_f_serve_attestation_duty(dvc, attestation_duty, dvc');                                                
+                        
+                    case AttConsensusDecided(id, decided_attestation_data) => 
+                        lemma_inv15_f_att_consensus_decided(dvc, id, decided_attestation_data, dvc');                                                
+                        
+                    case ReceviedAttesttionShare(attestation_share) =>                         
+                        lemma_inv15_f_listen_for_attestation_shares(dvc, attestation_share, dvc');                        
+                       
+                    case ImportedNewBlock(block) => 
+                        var dvc_mod := add_block_to_bn(dvc, block);
+                        lemma_inv15_add_block_to_bn(dvc, block, dvc_mod);
+                        assert inv15_body(dvc_mod);
+                        lemma_inv15_f_listen_for_new_imported_blocks(dvc_mod, block, dvc');                        
+                        assert inv15_body(dvc');
+                    
+                    case ResendAttestationShares =>                                                                      
+
+                    case NoEvent => 
+                        
+                }
+                
+            case AdeversaryTakingStep(node, new_attestation_share_sent, messagesReceivedByTheNode) =>
+                
+        }   
+    }  
 
 }
