src/dvspec/dafny/specification/dvc_spec.dfy
@@ -85,7 +85,7 @@ module DVCNode_Spec {
         attestation_duty: AttestationDuty,
         attestation_slashing_db: set<SlashingDBAttestation>
     ): ConsensusEngineState
-    requires id !in s.attestation_consensus_active_instances.Keys
+    // requires id !in s.attestation_consensus_active_instances.Keys
     {
         var acvc := AttestationConsensusValidityCheckState(
                     attestation_duty := attestation_duty,
@@ -298,7 +298,7 @@ module DVCNode_Spec {
         process: DVCNodeState,
         attestation_duty: AttestationDuty
     ): DVCNodeStateAndOuputs
-    requires forall ad | ad in process.attestation_duties_queue + [attestation_duty]:: ad.slot !in process.attestation_consensus_engine_state.attestation_consensus_active_instances.Keys
+    // requires forall ad | ad in process.attestation_duties_queue + [attestation_duty] :: ad.slot !in process.attestation_consensus_engine_state.attestation_consensus_active_instances.Keys
     {
         f_check_for_next_queued_duty(
             process.(
@@ -309,7 +309,7 @@ module DVCNode_Spec {
     }    
 
     function f_check_for_next_queued_duty(process: DVCNodeState): DVCNodeStateAndOuputs
-    requires forall ad | ad in process.attestation_duties_queue :: ad.slot !in process.attestation_consensus_engine_state.attestation_consensus_active_instances.Keys
+    // requires forall ad | ad in process.attestation_duties_queue :: ad.slot !in process.attestation_consensus_engine_state.attestation_consensus_active_instances.Keys
     decreases process.attestation_duties_queue
     {
         if  && process.attestation_duties_queue != [] 
@@ -346,7 +346,7 @@ module DVCNode_Spec {
     }         
 
     function f_start_next_duty(process: DVCNodeState, attestation_duty: AttestationDuty): DVCNodeStateAndOuputs
-    requires attestation_duty.slot !in process.attestation_consensus_engine_state.attestation_consensus_active_instances.Keys
+    // requires attestation_duty.slot !in process.attestation_consensus_engine_state.attestation_consensus_active_instances.Keys
     {
         DVCNodeStateAndOuputs(
             state :=  process.(
